pulse/share/steel/examples/pulse/bug-reports/ExistsSyntax.fst
@@ -6,8 +6,8 @@ module R = Pulse.Lib.Reference
 ```pulse
 fn some_function (r0:ref U8.t) (r1:ref U8.t) (#s:erased U8.t)
    requires 
-      R.pts_to r0 full_perm s **
-      exists (s1:U8.t). R.pts_to r1 full_perm s1
+      R.pts_to r0 s **
+      exists (s1:U8.t). R.pts_to r1 s1
    ensures
         emp
 {
@@ -21,8 +21,8 @@ fn some_function (r0:ref U8.t) (r1:ref U8.t) (#s:erased U8.t)
 ```pulse
 fn call_some_function (r0:ref U8.t) (r1:ref U8.t) (#s0:erased U8.t) (#s1:erased U8.t)
    requires
-     R.pts_to r0 full_perm s0 **
-     R.pts_to r1 full_perm s1
+     R.pts_to r0 s0 **
+     R.pts_to r1 s1
    ensures
      emp
 {
