pulse/share/steel/examples/pulse/bug-reports/IntroGhost.fst
@@ -10,15 +10,15 @@ module R = Pulse.Lib.Reference
 *)
 let my_inv (b:bool) (r:R.ref int) : vprop
   = exists_ (fun v -> 
-      R.pts_to r full_perm v ** 
+      R.pts_to r v ** 
       pure ( b == (v = 0) )
     )
 
 [@@expect_failure]
 ```pulse
 fn invar_introduces_ghost (r:R.ref int)
-  requires R.pts_to r full_perm 0
-  ensures R.pts_to r full_perm 1
+  requires R.pts_to r 0
+  ensures R.pts_to r 1
 {
   r := 0;
 
@@ -42,8 +42,8 @@ fn invar_introduces_ghost (r:R.ref int)
 [@@expect_failure]
 ```pulse
 fn exists_introduces_ghost (r:R.ref int)
-  requires R.pts_to r full_perm 0
-  ensures R.pts_to r full_perm 0
+  requires R.pts_to r 0
+  ensures R.pts_to r 0
 {
   r := 0;
 
@@ -62,8 +62,8 @@ fn exists_introduces_ghost (r:R.ref int)
 [@@expect_failure]
 ```pulse
 fn exists_with_witness_introduces_ghost (r:R.ref int)
-  requires R.pts_to r full_perm 0
-  ensures R.pts_to r full_perm 0
+  requires R.pts_to r 0
+  ensures R.pts_to r 0
 {
   r := 0;
 
@@ -84,8 +84,8 @@ fn exists_with_witness_introduces_ghost (r:R.ref int)
 *)
 ```pulse
 fn with_assert_OK (r:R.ref int)
-  requires R.pts_to r full_perm 0
-  ensures R.pts_to r full_perm 0
+  requires R.pts_to r 0
+  ensures R.pts_to r 0
 {
   r := 0;
 
