pulse/share/steel/examples/pulse/lib/Pulse.Lib.HigherReference.fsti
@@ -9,7 +9,7 @@ val ref (a:Type u#1) : Type u#0
 val pts_to (#a:Type) (r:ref a) (p:perm) (n:a) : vprop
 
 val alloc (#a:Type) (x:a)
-  : stt (ref a) emp (fun r -> pts_to r full_perm x)
+  : stt (ref a) emp (fun r -> pts_to r x)
 
 val ( ! ) (#a:Type) (r:ref a) (#n:erased a) (#p:perm)
   : stt a
@@ -18,11 +18,11 @@ val ( ! ) (#a:Type) (r:ref a) (#n:erased a) (#p:perm)
 
 val ( := ) (#a:Type) (r:ref a) (x:a) (#n:erased a)
   : stt unit
-        (pts_to r full_perm n)
-        (fun _ -> pts_to r full_perm (hide x))
+        (pts_to r n)
+        (fun _ -> pts_to r (hide x))
 
 val free (#a:Type) (r:ref a) (#n:erased a)
-  : stt unit (pts_to r full_perm n) (fun _ -> emp)
+  : stt unit (pts_to r n) (fun _ -> emp)
 
 val with_local
   (#a:Type u#1)
@@ -30,6 +30,6 @@ val with_local
   (#pre:vprop)
   (#ret_t:Type)
   (#post:ret_t -> vprop)
-  (body:(r:ref a) -> stt ret_t (pre ** pts_to r full_perm init)
-                               (fun v -> post v ** exists_ (pts_to r full_perm)))
+  (body:(r:ref a) -> stt ret_t (pre ** pts_to r init)
+                               (fun v -> post v ** exists_ (pts_to r)))
   : stt ret_t pre post
